added direct reductions - BSM n halting to MMA (1+n) halting - MMA (1+n) halting to MMA (1+n) halting on zero
Notice than the reduction MMA 0 halting to MMA 0 halting on zero
does not hold because the only program in MMA 0 is the empty list
which stop immediatly.

theories/MinskyMachines/MMA.v
@@ -77,12 +77,16 @@ Section MMA_problems.
 
   Definition MMA_PROBLEM n := (list (mm_instr (pos n)) * vec nat n)%type.
 
-  Definition MMA_HALTS_ON_ZERO {n} (P : MMA_PROBLEM n) := (1,fst P) // (1,snd P) ~~> (0,vec_zero).
-  Definition MMA_HALTING {n} (P : MMA_PROBLEM n) := (1,fst P) // (1,snd P) ↓.
+  Definition MMA_HALTS_ON_ZERO n (P : MMA_PROBLEM n) := (1,fst P) // (1,snd P) ~~> (0,vec_zero).
+  Definition MMA_HALTING n (P : MMA_PROBLEM n) := (1,fst P) // (1,snd P) ↓.
+
+  Global Arguments MMA_HALTS_ON_ZERO : clear implicits.
+  Global Arguments MMA_HALTING : clear implicits.
 
   Definition MMA2_PROBLEM := MMA_PROBLEM 2.
 
-  Definition MMA2_HALTS_ON_ZERO := @MMA_HALTS_ON_ZERO 2.
-  Definition MMA2_HALTING := @MMA_HALTING 2.
+  Definition MMA2_HALTS_ON_ZERO := MMA_HALTS_ON_ZERO 2.
+  Definition MMA2_HALTING := MMA_HALTING 2.
 
 End MMA_problems.
+
