theories/MinskyMachines/Reductions/MMA_to_MMA_zero.v
@@ -13,10 +13,14 @@ Require Import Undecidability.Synthetic.Definitions.
 Require Import Undecidability.Synthetic.ReducibilityFacts.
 
 From Undecidability.Shared.Libs.DLW Require Import utils pos vec sss subcode.
-From Undecidability.MinskyMachines Require Import MMA.
-From Undecidability.MinskyMachines Require MMA_to_MMA_zero.
+From Undecidability.MinskyMachines Require Import mma_defs mma_simul.
 
 Set Implicit Arguments.
 
-Theorem MMA2_MMA2_HALTS_ON_ZERO : MMA2_HALTING ⪯ MMA2_HALTS_ON_ZERO.
-Proof. apply MMA_to_MMA_zero.reduction. Qed.
+Theorem reduction n : MMA_HALTING (1+n) ⪯ MMA_HALTS_ON_ZERO (1+n).
+Proof.
+  apply reduces_dependent; exists.
+  intros (P,v).
+  destruct mma2_simulator with n 1 P as (Q & HQ).
+  exists (Q,v); apply HQ.
+Qed. 
